
> Not to be confused with *[[regular local rings]]* in [[commutative algebra]].

+-- {: .rightHandSide}
+-- {: .toc .clickDown tabindex="0"}
###Context###
#### Algebra
+--{: .hide}
[[!include higher algebra - contents]]
=--
=--
=--


\tableofcontents

## Idea

A *von Neumann regular ring* is a [[ring]] $A$ (not necessarily [[commutative ring|commutative]]) such that any of these equivalent conditions hold:

1. For every [[element]] $a \in A$ there exists $x \in A$ satisfying

$$
  a
  \;=\;
  a \, x \, a
  \,.
$$

2. For every $a \in A$ there is an idempotent $e \in A$ such that $A a = A e$.  In other words, every [[principal ideal|principal]]  [[left ideal]] of $A$ is generated by an idempotent.

3. For every $a \in A$ there is an [[idempotent]] $e \in A$ such that $a A = e A$.  In other words, every principal [[right ideal]] of $A$ is generated by an idempotent.

4. Every principal left ideal of $A$ is a direct summand of the left $A$-module $A$.

5. Every  principal right ideal of $A$ is a direct summand of the right $A$-module $A$.

6. Every left $A$-module is [[flat module|flat]].

7.  Every right $A$-module is [[flat module|flat]].

To illustrate the use of the rather curious-looking equation $a = a x a$, consider this:

\begin{lemma}
Suppose $a \in A$.  If for some $x \in A$ we have $a = a x a$, then $e = a x$ is idempotent and $a A = e A$. Conversely, if $a A = e A$ for some idempotent $e \in A$, then $a = a x a$ for some $x \in A$, and we can take $e = a x$.
\end{lemma}

\begin{proof} For the first implication, suppose for some $x \in A$ we have $a = a x a$.   Then $a x = a x a x$ so $e = a x$ is idempotent, and we just need to show $a A = e A$.   Since $e = a x$ we have $e A \subseteq a A$.   On the other hand, since $ a = a x a = e a$ we have $a A \subseteq e A$.

For the converse implication, suppose $a A = e A$ for some idempotent $e$.  This is equivalent to the conjunction of three conditions: $e \in a A$, $a \in e A$, and $e^2 = e$.      The first condition says $e = a x$ for some $x \in A$.  The second condition says $a = e y$ for some $y \in A$, which by the third condition implies $e a = e e y = e y = a$, which by the first implies $a x a = a$, as desired.
\end{proof}

## References

* Wikipedia, *[Von Neumann regular ring](https://en.wikipedia.org/wiki/Von_Neumann_regular_ring)*

Von Neumann regular rings were introduced by von Neumann in 1936 in his work on the algebraic approach to quantum mechanics:

* J. von Neumann, On Regular Rings, Proc. Natl. Acad. Sci. U.S.A. 22 (1936) 707-713.   ([web](https://doi.org/10.1073/pnas.22.12.707))

[[!redirects von Neumann regular rings]]
