# Bicategories of relations
* tic
{: toc}


## Idea

A *bicategory of relations* is a [[(1,2)-category]] which behaves like the 2-category of internal [[relations]] in a [[regular category]].  The notion is due to Carboni and Walters.


## Definition

[Note: in this article, the direction of composition is diagrammatic (i.e., "anti-Leibniz"). 

A **bicategory of relations** is a [[cartesian bicategory]] which is [[locally posetal 2-category|locally posetal]] and moreover in which for every object $X$, the [[diagonal morphism|diagonal]] $\Delta\colon X\to X\otimes X$ and [[codiagonal]] $\nabla\colon X\otimes X\to X$ satisfy the [[Frobenius condition]]:
$$\nabla\Delta = (1\otimes \Delta)(\nabla \otimes 1).$$

Of course, in the locally posetal case the definition of cartesian bicategory simplifies greatly: it amounts to a symmetric monoidal [[Pos]]-[[enriched category]] for which every object carries a commutative [[comonoid]] structure, for which the structure maps $\Delta_X: X \to X \otimes X$, $\varepsilon_X: X \to 1$ are [[left adjoint]] 1-morphisms, and for which every morphism $R: X \to Y$ is a colax morphism of comonoids in the sense that the following inequalities hold: 

$$R \Delta_Y \leq \Delta_{X \otimes X} (R \otimes R), \qquad R \varepsilon_Y \leq \varepsilon_X.$$

We remark that such structure is unique when it exists (being a cartesian bicategory is a property of, as opposed to structure on, a bicategory). The [[tensor product]] $\otimes$ behaves like the ordinary product of [[relation]]s. Note this is not a cartesian product in the sense of the usual universal property; nevertheless, it is customary to write it as a product $\times$, and we follow this custom below. It does become a cartesian product if one restricts to the subcategory of left adjoints (called _maps_), which should be thought of as functional relations. 

## Properties

We record a few consequences of this notion. 

+-- {: .num_prop} 
######Proposition 
(Separability condition) $\Delta\nabla = 1$.
=-- 

+-- {: .proof} 
######Proof
In one direction, we have the 2-cell $1 \leq \Delta\nabla$ which is the unit of the adjunction $\Delta \dashv \Delta_* = \nabla$. In the other direction, there is an adjunction $\varepsilon \dashv \varepsilon_*$ between the counit and its dual, and the unit of this adjunction is a 2-cell $1 \leq \varepsilon\varepsilon_*$, from which we derive 

$$\Delta\nabla = \Delta\Delta_* \leq \Delta (1 \times \varepsilon)(1 \times \varepsilon_*)\Delta_* = 1$$ 

where the last equation follows from the equation $\Delta(1 \times \varepsilon) = 1$ and its dual $(1 \times \varepsilon_*)\Delta_* = 1$. 
=--

+-- {: .num_prop}
######Proposition 
(Dual Frobenius condition) $\nabla \Delta = (\Delta \times 1)(1 \times \nabla)$.
=-- 

+-- {: .proof} 
######Proof
The locally full subcategory whose 1-cells are _maps_ (= left adjoints) has finite products, in particular a symmetry involution $\sigma$ for which 

$$\Delta_X \sigma_{X X} = \Delta_X$$

Additionally, the right adjoint $\sigma_{X Y *}$ is the inverse $\sigma_{X Y}^{-1} = \sigma_{Y X}$. Hence the equation above is mated to $\sigma_{X X} \nabla_X = \nabla_X$, and we calculate 

$$\array{
\nabla_X \Delta_X & = & \sigma_{X X}\nabla_X \Delta_X \sigma_{X X} \\
 & = & \sigma_{X X} (1 \times \Delta_X)(\nabla_X \times 1) \sigma_{X X} \\
 & = & (\Delta_X \times 1_X) \sigma_{X \times X, X} \sigma_{X \times X, X} (1_X \times \nabla_X) \\
 & = & (\Delta_X \times 1_X) (\sigma_{X X} \times 1) (1 \times \sigma_{X X}) (1 \times \nabla_X) \\
 & = & (\Delta_X \times 1_X)(1_X \times \nabla_X)
}$$ 

which gives the dual equation. 
=--

+-- {: .num_theorem}
######Theorem
In a bicategory of relations, each object is dual to itself, making the bicategory a compact closed bicategory. 
=-- 

+-- {: .proof} 
######Proof
Both the unit and counit of the desired adjunction $X \dashv X$ are given by equality predicates: 

$$\eta_X = (1 \stackrel{\varepsilon_*}{\to} X \stackrel{\Delta}{\to} X \times X) \qquad \theta_X = (X \times X \stackrel{\nabla}{\to} X \stackrel{\varepsilon}{\to} 1)$$

One of the triangular equations follows from the commutative diagram 

$$\array{
X & \stackrel{1 \times \varepsilon_*}{\to} & X \times X & \stackrel{1 \times \Delta}{\to} & X \times X \times X \\
 & {}_1\searrow & \downarrow \mathrlap{\nabla} & & \downarrow \mathrlap{\nabla \times 1} \\
 & & X & \overset{\Delta}{\to} & X \times X \\
 & &  & {}_{1}\searrow & \downarrow \mathrlap{\varepsilon \times 1} \\
 & & & & X
}$$

where the square expresses a Frobenius equation. The other triangular equation uses the dual Frobenius equation. 
=--

The compact closure allows us to define the opposite of a relation $R: X \to Y$ as the 1-morphism mate: 

$$R^{op} = (Y \stackrel{1_Y \times \eta_X}{\to} Y \times X \times X \stackrel{1_Y \times R \times 1_X}{\to} Y \times Y \times X \stackrel{\theta_Y \times 1_X}{\to} X)$$ 

In this way, a bicategory of relations becomes a [[dagger-compact category|â€ -compact]] $Pos$-enriched category. 

Recall (again) that a **map** in the bicategory of relations is the same as a 1-cell that has a right adjoint. 

+-- {: .num_prop #strict} 
###### Proposition 
If $f \colon X \to Y$ is a map, then $f$ is a strict morphism of comonoids. 
=-- 

+-- {: .proof} 
###### Proof 
If $g$ is the right adjoint of $f$, we have $\Delta_X g \leq (g \times g)\Delta_Y$ since $g$, like any morphism, is a lax comonoid morphism. But this 2-cell is mated to a 2-cell $(f \times f)\Delta_X \to \Delta_Y f$, inverse to the 2-cell $\Delta_Y f \to (f \times f)\Delta_X$ that comes for free. So $f$ preserves comultiplication strictly. A similar argument shows $f$ preserves the counit strictly. 
=-- 

+-- {: .num_prop}
###### Proposition 
If $f \colon X \to Y$ is a map, then $f^{op}: Y \to X$ equals the right adjoint $f_\ast$. 
=-- 

+-- {: .proof} 
###### Proof 
The proof is much more perspicuous if we use [[string diagram|string diagrams]]. But the key steps are given in two strings of equalities and inequalities. The first gives a counit for $f \dashv f^{op}$, and the second gives a unit. We have 

$$\array{
f f^{op} & \stackrel{0}{=} & f \circ (\varepsilon_Y \times 1)(\nabla_Y\times 1)(1 \times f \times 1)(1 \times \Delta_X)(1 \times \varepsilon_X_\ast) \\
& \stackrel{1}{=} & (\varepsilon_Y \times 1)(\nabla_Y \times 1)(1 \times f \times f)(1 \times \Delta_X)(1 \times \varepsilon_X_\ast) \\ 
 & \stackrel{2}{=} & (\varepsilon_Y \times 1)(\nabla_Y \times 1)(1 \times \Delta_Y)(1 \times f)(1 \times \varepsilon_X_\ast)\\ 
 & \stackrel{3}{\leq} & (\varepsilon_Y \times 1)(\nabla_Y \times 1)(1 \times \Delta_Y)(1 \times \varepsilon_Y_\ast) \\
 & \stackrel{4}{=} & (\varepsilon_Y \times 1)\Delta_Y \nabla_Y(1 \times \varepsilon_Y_\ast) \\
 & \stackrel{5}{=} & 1_Y
}$$ 

where (0) uses the definition of $f^{op}$, (1) uses properties of monoidal categories, (2) uses the fact that $f$ strictly preserves comultiplication, (3) is mated to the fact that $f$ laxly preserves the counit, (4) is a Frobenius condition, and (5) uses comonoid and dual monoid laws. We can also "almost" run the same calculation backwards to get the unit: 

$$\array{
1_X & \stackrel{0}{=} & (\varepsilon_X \times 1)\Delta_X \nabla_X(1 \times \varepsilon_X_\ast) \\ 
 & \stackrel{1}{=} & (\varepsilon_X \times 1)(\nabla_X \times 1)(1 \times \Delta_X)(1 \times \varepsilon_X_\ast) \\
 & \stackrel{2}{=} & (\varepsilon_Y \times 1)(f \times 1)(\nabla_X\times 1)(1 \times \Delta_X)(1 \times \varepsilon_X_\ast) \\ 
 & \stackrel{3}{\leq} & (\varepsilon_Y \times 1)(\nabla_Y \times 1)(f \times f \times 1)(1 \times \Delta_X)(1 \times \varepsilon_X_\ast) \\ 
 & \stackrel{4}{=} & (\varepsilon_Y \times 1)(\nabla_Y \times 1)(1 \times f \times 1)(1 \times \Delta_X)(1 \times \varepsilon_X_\ast) \circ f \\
 & \stackrel{5}{=} & f^{op} f
}$$ 

where (0) uses comonoid and dual monoid laws, (1) uses a Frobenius condition, (2) uses the fact that $f$ preserves the counit, (3) is mated to the fact that $f$ laxly preserves comultiplication, (4) uses properties of monoidal categories, and (5) uses the definition of $f^{op}$. 
=-- 

In fact, what this proof really proves is a converse of the earlier [proposition](#strict): 

+-- {: .num_prop}
###### Proposition 
If $f$ is a strict comonoid morphism, then $f$ has a right adjoint: $f \dashv f^{op}$. 
=-- 

+-- {: .num_prop}
######Proposition
If $f, g: X \to Y$ are maps and $f \leq g$, then $f = g$. Thus, the locally full subcategory whose morphisms are maps is locally discrete (the hom-posets are discrete). 
=-- 

+-- {: .proof} 
######Proof 
A 2-cell inequality $\alpha: f \leq g$ is mated to a inequality $\alpha_*: g_* \leq f_*$. On the other hand, whiskering $1_Y \times \alpha \times 1_X$ with $1_Y \times \eta_X$ and $\theta_Y \times 1_X$, as in the construction of opposites above, gives $\alpha^{op}: f^{op} \leq g^{op}$. Since $f^{op} = f_*$ and $g^{op} = g_*$, we obtain $f^{op} = g^{op}$, and because $f^{op op} = f$, we obtain $f = g$. 
=--

## The Beck-Chevalley condition 

Bicategories of relations $\mathbf{B}$ satisfy a Beck-Chevalley condition, as follows. Let $Prod(B_0)$ denote the free category with finite products generated by the set of objects of $\mathbf{B}$. According to the results at [[free cartesian category]], $Prod(B_0)$ is finitely complete. 

Since $Map(\mathbf{B})$ has finite products, there is a product-preserving functor $\pi: Prod(B_0) \to \Map(\mathbf{B})$ which is the identity on objects. Again, according to the results of [[free cartesian category]], we have the following result. 

+-- {: .num_lemma}
###### Lemma 
If a diagram in $Prod(B_0)$ is a pullback square, then application of $\pi$ to that diagram is a pullback square in $Map(\mathbf{B})$. 
=--

Let us call pullback squares of this form in $Map(\mathbf{B})$ _product-based_ pullback squares. 

+-- {: .num_prop}
######Proposition 
Given a product-based pullback square 
$$\array{
W & \stackrel{h}{\to} & X \\
k \downarrow & & \downarrow f \\
Y & \underset{g}{\to} & Z
}$$
in $Map(\mathbf{B})$, the Beck-Chevalley condition holds: $h_* k = f g_*$. 
=-- 

See Brady-Trimble for further details. The critical case to consider is the pullback square 

$$\array{
X & \overset{\Delta}{\to} & X \times X \\
\mathllap{\Delta} \downarrow & & \downarrow \mathrlap{\Delta \times 1} \\
X \times X & \underset{1 \times \Delta}{\to} & X \times X \times X
}$$

where the Beck-Chevalley condition is exactly the Frobenius condition. 

One way of interpreting this result is by viewing $\mathbf{B}$ as a hyperdoctrine or monoidal fibration over $Prod(B_0)$, where the fiber over an object $B$ is the local hom-poset $\hom(B, 1)$. Each $f: A \to B$ in the base induces a pullback functor, by precomposing $R: B \to 1$ with $\pi(f): A \to B$ in $Map(\mathbf{B})$. Existential quantification is interpreted by precomposing with right adjoints $\pi(f)_*$. The Beck-Chevalley condition exerts compatibility between quantification and pullback/substitution functors. 

## Relation to allegories 

Any bicategory of relations is an [[allegory]]. Recall that an allegory is a $Pos$-enriched $\dagger$-category whose local homs are meet-semilattices, satisfying Freyd's modular law: 

$$R S \cap T \leq (R \cap T S^{op})S$$ 

A proof of the modular law is given in the blog post by R.F.C. ("Bob") Walters referenced below. 

In fact, we may prove a little more: 

+-- {: .num_theorem} 
######Theorem 
The notion of bicategory of relations is equivalent to the notion of unitary pretabular allegory. 
=-- 

+-- {: .proof} 
######Proof 
A bicategory of relations has a unit $1$ in the sense of allegories: 

* $1$ is a partial unit: we have $\varepsilon_1 = id_1: 1 \to 1$, and for any $R: 1 \to 1$ we have $R = R\varepsilon_1 \leq \varepsilon_1 = id_1$. 

* Any object $X$ is the source of a map $\varepsilon_X: X \to 1$, which being a map is entire. Thus $1$ is a unit. 

A bicategory of relations is also pretabular, for the maximal element in $\hom(X, Y)$ is tabulated as $(\pi_X)_* \pi_Y$, where $\pi_X$, $\pi_Y$ are the product projections for $X \times Y$. 

In the other direction, suppose $\mathbf{A}$ is a unitary pretabular allegory.  By theorem 1.6 of Carboni--Walters, $\mathbf{A}$ is a [[Cartesian bicategory]] if:

* $Map(\mathbf{A})$ has finite products.

* $\mathbf{A}$ has local finite products, and $id_1$ is the top element of $\mathbf{A}(1,1)$.

* The tensor product defined as
$$ R \otimes S =  (p R p_*) \cap (p' S p'_*) $$
is functorial, where $p$ and $p'$ are the appropriate product projections.

For the first condition, the existence of a unit $1$ implies that $1$ is terminal in $Map(\mathbf{A})$, and the tabulation of the top element of $\mathbf{A}(X,Y)$ is the product cone $X \leftarrow X \times Y \to Y$.  For the second, local meets are given as part of the allegory structure, and the definition of a unit object gives top elements and the second part of the condition.

The third condition is a little trickier.  For identity morphisms, it says that $p p_* \cap p' p'_* = 1$, which is true because $(p,p')$ tabulates the top element of the relevant hom set.  Now suppose that $R, S \colon X \to Y$ and $R', S' \colon Y \to Z$.  The composition condition for the tensor product requires that
$$ p R R' p_* \cap p' S S' p'_*
   = (p R p_* \cap p' S p'_*) (p R' p_* \cap p' S' p'_*) $$
We may interpret the LHS as
$$ (x',z')^* (\exists y. z^* R x y \wedge x^* R' y z) \wedge (x,z)^* (\exists y'. z'^* S x' y' \wedge x'^* S' y' z')
$$
and the right as
$$
\exists y, y'. (z,z')^* ((x',y')^* R x y \wedge (x,y)^*S x' y') \wedge (x,x')^* ((y',z')^* R' y z \wedge (y,z)^* S' y' z')
$$
where $x^*, (x,y,\ldots)^*$ etc. represent pullback along (i.e. composition with) a product projection. But recall from [[allegory]] that existential formulas may be interpreted equally as either compositions or more complicated morphisms involving product projections and diagonals.  Applying this to the morphisms above, the result we want follows from [[Frobenius reciprocity]], which is a special case of the modular law, and some [[Beck-Chevalley conditions]]:
$$
\begin{aligned}
& (x',z')^* (\exists y. z^* R x y \wedge x^* R' y z) \wedge (x,z)^* (\exists y'. z'^* S x' y' \wedge x'^* S' y' z') \\
& = (\exists y. (z,x',z')^* R x y \wedge (x,x',z')^* R' y z) \wedge (\exists y'. (x,z,z')^* S x' y' \wedge (x,z,x')^* S' y' z')  \\
& = \exists y. ((z,x',z')^* R x y \wedge (x,x',z')^* R' y z \wedge y^* \exists y'. (x,z,z')^* S x' y' \wedge (x,z,x')^* S' y' z')  \\
& = \exists y. ((z,x',z')^* R x y \wedge (x,x',z')^* R' y z \wedge \exists y'. y^* ((x,z,z')^* S x' y' \wedge (x,z,x')^* S' y' z')) \\
& = \exists y, y'. (y'^*((z,x',z')^* R x y \wedge (x,x',z')^* R' y z) \wedge y^* ((x,z,z')^* S x' y' \wedge (x,z,x')^* S' y' z')) \\
& = \exists y, y'. ((y,z,x',z')^* R x y \wedge (x,y,x',z')^* R' y z \wedge ((x,y,z,z')^* S x' y' \wedge (x,y,z,x')^* S' y' z')) \\
& = \exists y, y'. (z,x',y',z')^* R x y \wedge  (x,y,z,z')^* S x' y' \wedge (x,x',y',z')^* R' y z \wedge (x,y,z,x')^* S' y' z') \\
& = \exists y, y'. (z,z')^* ((x',y')^* R x y \wedge (x,y)^*S x' y') \wedge (x,x')^* ((y',z')^* R' y z \wedge (y,z)^* S' y' z')
\end{aligned}
$$
The Beck--Chevalley swap in the second line holds because there $\exists$ is expressed by post-composition with a projection, and pullback/substitution by precomposition, and these automatically commute in a 2-category.  That in line 4 is valid because it amounts to the identity $\epsilon_{Y'}\epsilon^o_Y = p'_* p$, where $p$ and $p'$ are the projections out of $Y \times Y'$.


Finally, the modular law implies [[Frobenius reciprocity]], which implies the Frobenius laws as shown at _loc. cit._

=--


## See also

Other attempted axiomatizations of the same idea "something that acts like the category of relations in a regular category" include:

* [[allegories]]

* [[1-category equipped with relations]]


## References

* Carboni and Walters, "Cartesian Bicategories, I"

* [blog post](http://rfcwalters.blogspot.com/2009/10/categorical-algebras-of-relations.html) showing that any bicategory of relations is an [[allegory]]. Indeed, a bicategory of relations is equivalent to a unitary pretabular allegory.


[[!redirects bicategories of relations]]