In its usual form, the Eckmann--Hilton argument shows that a [[monoid]] or [[group object]] [[internalization|in]] the category of monoids or [[Grp|groups]] is [[abelian group|commutative]]. In other terms, if a set is equipped with two monoid structures, such that one is a homomorphism for the other, then the two structures coincide and the resulting monoid is commutative.

An even more general version is this:  If a set is equipped with two binary operations with [[identity]], as long as they commute with each other in the sense that one is (with respect to the other) a homomorphism of sets with binary operations, then everything else follows:
1.  the other is also a homomorphism with respect to the first;
1.  each also preserves the other\'s identity;
1.  the identities are the same;
1.  the operations are the same;
1.  the operation is commutative;
1.  the operation is associative.

# Proof #

The basic equation that we have (that one operation $*$ is a homomorphism with respect to another operation $\circ$) is
$$ (a \circ b) * (c \circ d) = (a * c) \circ (b * d) .$$
We prove the above list of results in order:

1.  Simply read the basic equation backwards to see that $\circ$ is a homomorphism with respect to $*$.

1.  Now if $1_*$ is the identity of $*$ and $1_\circ$ is the identity of $\circ$, we have
$$ 1_\star \circ 1_\star = (1_\star \circ 1_\star) * 1_\star = (1_\star \circ 1_\star) * (1_\star \circ 1_\circ) = (1_\star * 1_\star) \circ (1_\star * 1_\circ) = 1_\star \circ 1_\circ = 1_\star .$$
A similar argument proves the other half.

1.  Then
$$ 1_\star = 1_\star * 1_\star = (1_\star \circ 1_\circ) * (1_\circ \circ 1_\star) = (1_\star * 1_\circ) \circ (1_\circ * 1_\star) = 1_\circ \circ 1_\circ = 1_\circ ,$$
so the identities are the same; we will now write this identity simply as $1$.

1.  Now
$$ a * b = (a \circ 1) * (1 \circ b) = (a * 1) \circ (1 * b) = a \circ b ,$$
so the operations are the same; we will write them both with concatenation.

1.  Then
$$ a b = (1 a) (b 1) = (1 b) (a 1) = b a ,$$
so this operation is commutative.

1.  Finally,
$$ (a b) c = (a b) (1 c) = (a 1) (b c) = a (b c) ,$$
so the operation is associative.

Note that if you start with the slick monoid-in-$Mon$ approach, then only (4&5) need to be shown; the others are part of the hypothesis.  This classic form of the Eckmann--Hilton argument may be combined into a single calculation:
$$ a * b = (a \circ 1) * (1 \circ b) = (a * 1) \circ (1 * b) = a \circ b = (1 * a) \circ (b * 1) = (1 * b) \circ (a * 1) = b * a ,$$
where the desired results involve the first, middle, and last expressions.

# Corollaries #

A $2$-[[k-tuply monoidal n-category|tuply monoidal]] $0$-[[0-category|category]], if defined as a [[pointed object|pointed]] $2$-[[k-tuply connected n-category|tuply connected]] [[bicategory]] is also the same as an abelian monoid.

A $2$-tuply monoidal $1$-[[1-category|category]], if defined as a pointed $2$-tuply connected [[tricategory]], is the same as a [[braided monoidal category]].

Every [[homotopy group]] $\pi_n$ for $n \geq 2$ is [[abelian group|abelian]].

#References#

*The argument is really much more interesting if proved (and applied) geometrically, as in these VIDEO lectures from the Catsters:
 *  [Eckmann-Hilton 1](http://www.youtube.com/watch?v=Rjdo-RWQVIY);
 *  [Eckmann-Hilton 2](http://www.youtube.com/watch?v=wnRqo7UHa-k).

*For higher analogues see 
 * (within the discussion of commutative algebraic monads) N. Durov, New approach to Arakelov geometry, [arXiv:0704.2030](http://arxiv.org/abs/0704.2030)
 * M. A. Batanin, The Eckmann-Hilton argument and higher operads,  Adv. Math.  217  (2008),  no. 1, 334--385; [arXiv:math.CT/0207281](http://arxiv.org/abs/math/0207281)