new test

$$
  \begin{aligned}
   & e_7 (e_6 (e_5 (e_4 (e_3 (\underset{-e_4}{\underbrace{e_2 e_1}})))))
   \\
   & =
   - e_7 (e_6 (e_5 (e_4 (\underset{e_6}{\underbrace{e_3 e_4}}))))
   \\
   & =
   - e_7 (e_6 (e_5 (\underset{e_3}{\underbrace{e_4 e_6}})))
   \\
   & =
   - e_7 (e_6 (\underset{-e_2}{\underbrace{e_5 e_3}}))
   \\
   & =
   + e_7 (\underset{-e_7}{\underbrace{e_6 e_2}})
   \\
   & =
   - \underset{= -1}{\underbrace{e_7 e_7}}
   \\
   & =
   + 1
  \end{aligned}
$$