[For convenience we assume below that $M$ is a $G$-module, it does not in general have to be abelian and it suffices to have it a $G$-group.]


Suppose $G$ is a [[group]] and $M$ a $G$-[[module]] and let $\delta : G \to M$ be a __derivation__. This means $\delta(g_1g_2) = \delta(g_1) +g_1\delta(g_2)$ for all $g_1, g_2 \in G$.  (Note: *not* $\delta(g_1)g_2 + g_1\delta(g_2)$ as for the other notion of [[derivation]].)

For calculations, the following lemma is very valuable, although very simple to prove.

+-- {: .un_lemma}
###### Lemma

If  $\delta : G \to M$ is a derivation, then

1. $ \delta(1_G) = 0$;

2. $\delta(g^{-1}) = -g^{-1}\delta(g)$ for all $g \in G$;

3. for any $g \in G$ and $n\geq 1$, 

   $$\delta(g^n) = (\sum^{n-1}_{k=0}g^k)\delta(g).$$
=--

+-- {: .proof}
###### Proof
As was said, these are easy to prove.

$\delta(g) = \delta(1g) + 1\delta(g)$, so $\delta(1)= 0$, and hence (1); then 

$$\delta(1) = \delta(g^{-1}g) = \delta(g^{-1}) + g^{-1}\delta(g)$$ 

to get (2), and finally induction to get (3).
=--

###Remark:

The [[Fox derivatives]] are examples.  It is worth noting that this lemma allows a simplification of the conditions given there (as noted there).

###Example (using the [[Fox derivative]] w.r.t a generator)

 Let $X = \{u,v\}$, with $r \equiv u v u v^{-1} u^{-1} v^{-1} \in F = F(u,v),$ then


$$ \frac{\partial r}{\partial u} = 1 + u v - u v u v^{-1} u^{-1},$$


$$ \frac{\partial r}{\partial v} = u - u v u v^{-1} -  u v u v^{-1} u^{-1} v^{-1}.$$
This relation, $r$, is the typical [[braid group]] relation, here in $Br_3$.


