Various people have "challenged" category theorists to write down a fully formal presentation of ETCS. We will do so here. 

There will be no pretense to elegance or other aesthetic criteria such as efficiency or lack of redundancy. At a first pass we will do things in a quick and dirty way, and with luck there will be various polishings of this entry as time passes. 

We assume familiarity with the standard notion of a (finitary) first-order theory with equality. Such theories are typically presented in terms of a signature consisting of function and predicate symbols, together with axioms each of which is a closed formula in the first-order language generated by the signature. Standard logical conventions are followed; for example, it is common to state axioms as formulas $P(x_1, \ldots, x_n)$ in which some of the variables $x_i$ may appear freely, but in such cases it is implicit that such variables are bound by universally quantifiers at the head of the formula. 

To make the exposition more readable, the theory will be presented in fragments, together with some explanations (in parentheses) which do not belong to the formal theory, but which may aid comprehension. 

## The theory of categories 

The signature of $Th(Cat)$ consists of 

* Unary function symbols $s$, $t$; 

* A ternary predicate $c$. 

(The theory of categories is commonly presented as a two-sorted theory, with an object sort and a morphism sort. Here we instead use a single-sorted theory, whose terms are intended to be interpreted as _morphisms_ of a category. We generally use letters $f, g, h, \ldots$ for variable terms. If $e$ is any term, then the intended interpretation of $s(e)$ is: the identity morphism of the domain of $e$, and $t(e)$ means the identity morphism of the codomain of $e$. The intended interpretation of $c(f, g, h)$ is that $h = f \circ g$.) 

The axioms of $Th(Cat)$ are as follows:  

1. $\vdash (s s(f) = s(f) = t s (f)) \wedge (t t(f) = t(f) = s t(f))$. 

1. $c(f, g, h) \vdash s(f) = t(g) \wedge t(f) = t(h) \wedge s(g) = s(h)$

1. (Composition is well-defined) $c(f, g, h) \wedge c(f, g, h') \vdash h = h'$

1. $s(f) = t(g) \vdash \exists_h c(f, g, h)$

1. (Identity laws) $\vdash c(f, s(f), f) \wedge c(t(f), f, f)$

1. (Associativity) $c(f, g, j) \wedge c(g, h, k) \vdash (c(j, h, m) \Leftrightarrow c(f, k, m))$


