
+-- {: .rightHandSide}
+-- {: .toc .clickDown tabindex="0"}
###Context###
#### Homological algebra
+--{: .hide}
[[!include homological algebra - contents]]
=--
=--
=--

#Contents#
* table of contents
{:toc}

## Idea

For $0 \to A \to B \to C \to 0$ a [[short exact sequence]] of [[cochain complexes]] in an [[abelian category]] $\mathcal{A}$, the corresponding [[cohomology long exact sequence]]

$$
  \cdots \to H^n(A) \to H^n(B) \to H^n(C) \stackrel{\delta}{\to} H^{n+1}(A) \to H^{n+1}(B) \to H^{n+1}(C) \to \cdots
$$

has in every third step a morphism $\delta$ that shifts cohomological degree. This is called a _connecting homomorphism_ . 

If $\mathcal{A}$ is [[Freyd-Mitchell embedding theorem|realized]] as some $R$[[Mod]], then the connecting homomorphism is explicitly constructed as follows:

for $[c]_C \in H^n(C)$ the class of a closed element $c$, by surjectivity of $B \to C$ there is an element $\hat c \in B$ mapping to it. This need not be closed anymore, but of course $d_B \hat c$ is. By the fact that $B \to C$ is a chain map we have that the image of $d_B \hat c$ in $B$ vanishes. Therefore by the exactness of the sequence the element $d_B \hat c$ may be regarded as a closed element of $A$. The cohomology class $[d_B \hat c]_A$ of this is what the connecting homomorphism assigns to $[c]_C$:

$$
  \delta : [c]_C \mapsto [d_B\hat c]_A
  \,.
$$

This is indeed well defined, in that it is independent of the choice of $\hat c$: for $\hat c'$ another choice, we have that the difference $\hat c - \hat c'$ is in the kernel of $B \to C$ hence is in $A$. Then $d_B \hat c' = d_B \hat C + d_A(\hat c - \hat c')$. Hence $[d_B \hat c]_A = [d_B \hat c']_A$.


## Statement

+-- {: .num_theorem}
###### Theorem

Let $0 \to A_\bullet \stackrel{f}{\to} B_\bullet \stackrel{g}{\to} C_\bullet \to 0$
be a [[short exact sequence]] of [[chain complexes]] in some [[abelian category]] $\mathcal{A}$. Then for all $n \in \mathbb{Z}$ there are natural _connecting homomorphisms_ $\partial : H_n(C) \to H_{n-1}(A)$ such that we have a [[long exact sequence]] of the form

$$
  \cdots \stackrel{g}{\to}
  H_{n+1}(C)
  \stackrel{\partial}{\to}
  H_n(A)
  \stackrel{f}{\to}
  H_n(B)
  \stackrel{g}{\to}
  H_n(C)
  \stackrel{\partial}{\to}
  H_{n-1}(A)
  \stackrel{f}{\to}
  \cdots
$$

in [[chain homology]].

=--

+-- {: .proof}
###### Proof

A proof not using the [[Freyd-Mitchell embedding theorem]] can proceed as follows.

Applying the [[snake lemma]] to the [[commuting diagram]]

$$
  \array{
     && 0 && 0 && 0   
     \\
     && \downarrow && \downarrow && \downarrow 
     \\
     0 &\to& Z_n A &\to& Z_n B &\to & Z_n C
     \\
     && \downarrow && \downarrow && \downarrow 
     \\
     0 &\to& A_n &\to& B_n &\to & C_n &\to & 0 
     \\
     && \downarrow^{\mathrlap{d}} && \downarrow^{\mathrlap{d}} && \downarrow^{\mathrlap{d}}     
     \\
     0 &\to& A_{n-1} &\to& B_{n-1} &\to & C_{n-1} &\to& 0
     \\
     && \downarrow && \downarrow && \downarrow 
     \\
     0 &\to& \frac{A_{n-1}}{im(d)(A_n)} &\to& \frac{B_{n-1}}{im(d)(B_n)} &\to & \frac{C_{n-1}}{im(d)(C_n)} &\to & 0 
     \\
     && \downarrow && \downarrow && \downarrow 
     \\
     && 0 && 0 && 0     
  }
$$

shows that the rows in the commuting diagram


$$
  \array{
      && \frac{A_{n}}{im(d)(A_{n+1})} &\to& \frac{B_{n}}{im(d)(B_{n+1})} &\to & \frac{C_{n}}{im(d)(C_{n+1})} &\to & 0 
      \\
     && \downarrow^{\mathrlap{d}} && \downarrow^{\mathrlap{d}} && \downarrow^{\mathrlap{d}}     
     \\
     0 &\to& Z_{n-1} A &\stackrel{f}{\to}& Z_{n-1} B &\stackrel{g}{\to}& Z_{n-1} C
  }
$$

are [[exact sequences]]. Therefore applying the [[snake lemma]] to this, once more, yields the desired long exact sequence.

=--

## References

For instance section 1.3 of 

* [[Charles Weibel]], _[[An Introduction to Homological Algebra]]_


[[!redirects connecting homomorphisms]]
