
+-- {: .rightHandSide}
+-- {: .toc .clickDown tabindex="0"}
### Context
#### Differential geometry
+-- {: .hide}
[[!include synthetic differential geometry - contents]]
=--
=--
=--

# Contents
* table of contents
{: toc}

## Statement

The **chain rule** is the statement that [[differentiation]] $d : Diff \to Diff$  is a [[functor]] on [[Diff]]:

given two [[smooth function]]s between [[smooth manifold]]s $f : X \to Y$ and $g : Y \to Z$ we have

$$
  d(g \circ f) : 
  T X 
  \stackrel{d f}{\to}
  T Y 
  \stackrel{d g}{\to}
  T Z
  \,.
$$

If one thinks of a [[tangent vector]] $v \in T_x X$ to be an equivalence class of a smooth path $\gamma_v : [-\epsilon,\epsilon] \to X$, for some $\epsilon\gt 0$, with $\gamma(0) = x$, then the chain rule is the [[associativity]] of the composite

$$
  [-\epsilon,\epsilon] \stackrel{\gamma_v}{\to} X \stackrel{f}{\to} Y \stackrel{g}{\to} Z
  \,.
$$

Bracketed as $(g \circ f)\circ \gamma_v$ this represents $d(g \circ f)(v)$. Bracketed as $g \circ (f \circ \gamma_v)$ is represents $d g (d f (v))$.

Alternatively, in a context of [[synthetic differential geometry]] where with $D$ being the [[infinitesimal space|infinitesimal interval]] we may _identify_ $v$ with $v : D \to X$, the chain rule is the associativity of

$$
  D \stackrel{v}{\to} X \stackrel{f}{\to} Y \stackrel{g}{\to} Z
  \,.
$$


## Examples

### Elementary calculus

Let $X = Y = Z = \mathbb{R}$ the [[real line]]. Then the [[tangent bundle]] $T X$ is canonically identified with $\mathbb{R} \times \mathbb{R}$.

Given two functions, $f, g : \mathbb{R} \to \mathbb{R}$ their derivatives are traditionally regarded again as functions $f', g' : \mathbb{R} \to \mathbb{R}$, though strictly speaking we are to think of them as the maps

$$
  d f, d g : \mathbb{R} \times \mathbb{R} = T \mathbb{R}  \to T \mathbb{R}  = \mathbb{R} \times \mathbb{R}
$$

given by

$$
  d f : (x,v) \mapsto (f(x), v f'(x))
$$

and

$$
  d g : (x,v) \mapsto (g(x), v g'(x))
  \,.
$$

The composite

$$
  f (g \circ f) : \mathbb{R} \times \mathbb{R} = 
  T \mathbb{R} \to T \mathbb{R} = \mathbb{R} \times \mathbb{R}
$$

is therefore the map

$$
  d(g \circ f) : (x,v) \mapsto (f(x), v f'(x)) 
   \mapsto 
     (g(f(x)), v f'(x) g'(f(x)))
  \,.
$$

Therefore we have

$$
  (g \circ f)'(x) = f'(x) g'(f(x))
  \,.
$$

This is the form in which the chain rule is usually introduced in elementary calculus.

#### Remarks

While the chain rule is of great theoretical importance, it is completely unnecessary for the working out of derivatives of elementary functions in ordinary calculus (including the multivariable case).  Every result giving the derivative of an elementary function corresponds to a rule (along the lines of the [[product rule]]) for the operation of that function to any expression.  For example, instead of learning that
$$ \frac{\mathrm{d}}{\mathrm{d}x} (\sin x) = \cos x $$
and then applying both this fact *and* the chain rule to find the derivative of an expression of the form $\sin u$, just learn
$$ \frac{\mathrm{d}}{\mathrm{d}x} (\sin u) = \cos u \,\frac{\mathrm{d}u}{\mathrm{d}x} $$
and apply this rule directly; the original fact is the special case in which $u \coloneqq x$.  Even better, learn the rule as
$$ \mathrm{d}(\sin u) = \cos u \,\mathrm{d}u ;$$
then it applies without further modification to multivariable calculus (as well as implicit differentiation, related rates, integration by substitution, and other stock features of one-variable calculus).

The chain rule could still be used in the *proof* of this 'sine rule'.  Even so, it is quite possible to prove the sine rule directly (much as one proves the product rule directly rather than using the two-variable chain rule and the partial derivatives of the function $x, y \mapsto x y$).  In any case, the chain rule is not directly needed when working out specific derivatives.  As a *rule* of differentiation, the chain rule is needed only when an unspecified [[differentiable function]] $f$ appears, and then may be given in the form
$$ \frac{\mathrm{d}}{\mathrm{d}x} f(u) = f'(u) \,\frac{\mathrm{d}u}{\mathrm{d}x} $$
or
$$ \mathrm{d}f(u) = f'(u) \,\mathrm{d}u $$
to match other rules.

Although the chain rule is often written as
\[ \frac{\mathrm{d}y}{\mathrm{d}x} = \frac{\mathrm{d}y}{\mathrm{d}u} \,\frac{\mathrm{d}u}{\mathrm{d}x} ,\label{trivial} $$
this is an oversimplification.  Upon choosing an independent variable, it is possible (and easy) to give a rigorous definition of the [[differential]] $\mathrm{d}u$, and then (eq:trivial) is a triviality.  However, with such a definition of differential, (eq:trivial) is *not* the chain rule!  The reason is that, when (eq:trivial) is used as a mnemonic for the chain rule, ${\mathrm{d}u}/{\mathrm{d}x}$ uses $x$ as the independent variable, but ${\mathrm{d}y}/{\mathrm{d}u}$ uses $u$.  Either may be chosen to define differentials, but one must (a priori) be consistent.  Now, it so happens that the choice of independent variable is entirely irrelevant; differentials have the same meaning no matter which independent variable is used.  But *this* fact requires proof; *it* is the chain rule (or at least a prerequisite for using (eq:trivial) as the chain rule), and it is *not* a triviality.


[[!redirects chain rule]]
[[!redirects chain law]]
