
+-- {: .rightHandSide}
+-- {: .toc .clickDown tabindex="0"}
### Context
#### Type theory
+-- {: .hide}
[[!include type theory - contents]]
=--
=--
=--

# Contents
* table of contents
{: toc}

## Idea

In [[type theory]] a _function type_ $X \to Y$ for two [[types]] $X,Y$ is the [[type]] of [[functions]] from $X$ to $Y$. 

In a [[model]] of the type theory in [[categorical semantics]], this is an [[exponential object]]. In [[set theory]], it is a [[function set]]. In [[dependent type theory]], it is a special case of a [[dependent product type]].

## Definition

Like any type constructor in type theory, a function type is specified by rules saying when we can introduce it as a type, how to construct terms of that type, how to use or “eliminate” terms of that type, and how to compute when we combine the constructors with the eliminators.

The rule to build a function type is easy:

$$\frac{A\colon Type \qquad B \colon Type}{A\to B\colon Type}$$

### As a negative type

Function types are almost always defined as a [[negative type]].  In this presentation, primacy is given to the eliminators.  The natural eliminator of a function type says that we can *apply* it to any input:

$$\frac{f\colon A\to B \qquad a\colon A}{f(a) \colon B}$$

The constructor is then determined as usual for a negative type: to construct a term of $A\to B$, we have to specify how it behaves when applied to any input.  In other words, we should have a term of type $B$ containing a free variable of type $A$.  This yields the usual "$\lambda$-abstraction" constructor:

$$\frac{x\colon A\vdash b\colon B}{\lambda x.b\colon A\to B}$$

The [[β-reduction]] rule is the obvious one (the ur-example of all $\beta$-reductions), saying that when we evaluate a $\lambda$-abstraction, we do it by substituting for the bound variable.

$$(\lambda x.b)(a) \;\to_\beta\; b[a/x]$$

If we want an [[η-conversion]] rule, the natural one says that every function is a $\lambda$-abstraction:

$$ \lambda x.f(x) \;\to_\eta\; f$$

### As a positive type

It is also possible to present function types as a [[positive type]].  However, this requires a stronger metatheory, such as a [[logical framework]].  We use the same constructor ($\lambda$-abstraction), but now the eliminator says that to define an operation using a function, it suffices to say what to do in the case that that function is a lambda abstraction.

$$\frac{(x\colon A \vdash b\colon B) \vdash c\colon C \qquad f\colon A\to B}{funsplit(c,f)\colon C}$$

This rule cannot be formulated in the usual presentation of type theory, since it involves a "higher-order judgment": the context of the term $c\colon C$ involves a "term of type $B$ containing a free variable of type $A$".  However, it is possible to make sense of it.  In [[dependent type theory]], we need additionally to allow $C$ to depend on $A\to B$.

The natural $\beta$-reduction rule for this eliminator is

$$ funsplit(c, \lambda x.g) \;\to_\beta c[g/b] $$

and its $\eta$-conversion rule looks something like

$$ funsplit(c[\lambda x.b / g], f) \;\to_\eta\; c[f/g]. $$

Here $g\colon A\to B \vdash c\colon C$ is a term containing a free variable of type $A\to B$.  By substituting $\lambda x.b$ for $g$, we obtain a term of type $C$ which depends on "a term $b\colon B$ containing a free variable $x\colon A$".  We then apply the positive eliminator at $f\colon A\to B$, and the $\eta$-rule says that this can be computed by just substituting $f$ for $g$ in $c$.

### Positive versus negative

As usual, the positive and negative formulations are equivalent in a suitable sense.  They have the same constructor, while we can formulate the eliminators in terms of each other:

$$
\begin{aligned}
  f(a) &\coloneqq funsplit(b[a/x], f)\\
  funsplit(c, f) &\coloneqq c[f(x)/b]
\end{aligned}
$$

The conversion rules also correspond.

In dependent type theory, this definition of $funsplit$ only gives us a properly typed dependent eliminator if the negative function type satisfies $\eta$-conversion.  As usual, if it satisfies [propositional eta-conversion](/nlab/show/eta-conversion#Propositional) then we can transport along that instead---and conversely, the dependent eliminator allows us to prove propositional $\eta$-conversion.  This is the content of Propositions 3.5, 3.6, and 3.7 in [(Garner)](#GarnerSDP).


## Related concepts

* [[dependent product type]]
* [[lambda calculus]]

## References

* [[Richard Garner]], *On the strength of dependent products in the type theory of Martin-Löf*.
 {#GarnerSDP}

[[!redirects function type]]
[[!redirects function types]]
