## Definition 

+-- {: .un_def}
###### Definition 
A **monoidal monad** is a [[monad]] in the [[2-category]] of [[monoidal category|monoidal categories]], [[lax monoidal functor|lax monoidal functors]], and monoidal transformations. 
=-- 

The notion of monoidal monad is equivalent to a suitable general notion of _commutative monad_, as discussed at [[commutative algebraic theory]]. We explore this connection below. 

## Tensorial strengths and commutative monads 

As a preliminary, let $V$ be a monoidal category, and let $T \colon V \to V$ be a **strong** monad on $V$, meaning here that there are left and right [[tensorial strength|tensorial strengths]] 
$$\tau_{A, B} \colon A \otimes T(B) \to T(A \otimes B)$$

$$\,$$ 

$$\sigma_{A, B} \colon T(A) \otimes B \to T(A \otimes B).$$ 

which are suitably compatible with one another. The full set of coherence conditions may be summarized by saying $T$ preserves the two-sided monoidal action of $V$ on itself, in an appropriate 2-categorical sense. More precisely: the two-sided action of $V$ on itself is a [[lax functor]] of 2-categories  
$$\tilde{V} \colon B V \times (B V)^{op} \to Cat$$ 
($B V$ is the one-object 2-category associated with a monoidal category $V$, and $(B V)^{op}$ is the same 2-category but with 1-cell composition (= tensoring) in reverse order), and the two-sided strength means we have a structure of [[lax natural transformation]] $\tilde{V} \to \tilde{V}$. 

We remark that in the _symmetric_ monoidal setting, we will assume that the left and right strengths $\tau$ and $\sigma$ are related by the symmetry in the obvious way, by a commutative square 

$$\array{
A \otimes T(B) & \stackrel{\tau_{A, B}}{\to} & T(A \otimes B) \\
 ^\mathllap{c} \downarrow & & \downarrow^\mathrlap{T(c)} \\
T(B) \otimes A & \underset{\sigma_{B, A}}{\to} & T(B \otimes A)
}$$ 

where the $c$'s are instances of the symmetry isomorphism. 

+-- {: .un_def}
###### Definition 
Let $T \colon V \to V$ be a strong functor. A monad structure $(m \colon T T \to T, u: 1 \to T)$ is **commutative** if there is an equality of natural transformations $\alpha = \beta$ where 

* $\alpha$ is the composite 
$$T A \otimes T B \stackrel{\sigma_{A, T B}}{\to} T(A \otimes T B) \stackrel{T(\tau_{A, B})}{\to} T T(A \otimes B) \stackrel{m(A \otimes B)}{\to} T(A \otimes B).$$ 

* $\beta$ is the composite 
$$T A \otimes T B \stackrel{\tau_{T A, B}}{\to} T(T A \otimes B) \stackrel{T(\sigma_{A, B})}{\to} T T(A \otimes B) \stackrel{m(A \otimes B)}{\to} T(A \otimes B).$$ 
=-- 

## From monoidal monads to commutative monads 

Let $(T \colon V \to V, u \colon 1 \to T, m \colon T T \to T)$ be a monoidal monad, with structural constraints on the underlying functor denoted by 

$$\alpha_{A, B} \colon T(A) \otimes T(B) \to T(A \otimes B), \qquad \iota = u I: I \to T(I).$$ 

Define [[tensorial strength|strengths]] on both the left and the right by 

$$\tau_{A, B} = (A \otimes T(B) \stackrel{u A \otimes 1}{\to} T(A) \otimes T(B) \stackrel{\alpha_{A, B}}{\to} T(A \otimes B)),$$ 

$$\,$$ 

$$\sigma_{A, B} = (T(A) \otimes B \stackrel{1 \otimes u B}{\to} T(A) \otimes T(B) \stackrel{\alpha_{A, B}}{\to} T(A \otimes B)).$$ 

+-- {: .un_prop}
###### Proposition 
$(m \colon T T \to T, u \colon 1 \to T)$ is a commutative monad. 
=-- 

+-- {: .proof} 
###### Proof 
In fact, the two composites 

$$T A \otimes T B \stackrel{\sigma_{A, T B}}{\to} T(A \otimes T B) \stackrel{T(\tau_{A, B})}{\to} T T(A \otimes B) \stackrel{m(A \otimes B)}{\to} T(A \otimes B)$$ 

$$\,$$ 

$$T A \otimes T B \stackrel{\tau_{T A, B}}{\to} T(T A \otimes B) \stackrel{T(\sigma_{A, B})}{\to} T T(A \otimes B) \stackrel{m(A \otimes B)}{\to} T(A \otimes B)$$

are both equal to $\alpha_{A, B}$. We show this for the first composite; the proof is similar for the second. If $\alpha_T$ denotes the monoidal constraint for $T$ and $\alpha_{T T}$ the constraint for the composite $T T$, then by definition $\alpha_{T T}$ is the composite given by  
$$T T X \otimes T T Y \stackrel{\alpha_T T}{\to} T(T X \otimes T Y) \stackrel{T\alpha_T}{\to} T T(X \otimes Y)$$ 
and so, using the properties of monoidal monads, we have a commutative diagram 

$$\array{
 & & T T X \otimes T Y & \stackrel{\alpha_T}{\to} & T(T X \otimes Y) \\
 & ^\mathllap{u \otimes 1} \nearrow & \downarrow^\mathrlap{1 \otimes T u} & & \downarrow^\mathrlap{T(1 \otimes u)} \\
T X \otimes T Y & \stackrel{u \otimes T u}{\to} & T T X \otimes T T Y & \stackrel{\alpha_T T}{\to} & T(T X \otimes T Y) \\
 & ^\mathllap{1} \searrow & \downarrow^\mathrlap{m \otimes m} & \searrow^\mathrlap{\alpha_{T T}} & \downarrow^\mathrlap{T\alpha_T} \\
 & & T X \otimes T Y & & T T(X \otimes Y) \\
& & & ^\mathllap{\alpha_T} \searrow & \downarrow^\mathrlap{m} \\
 & & & & T(X \otimes Y)
}$$ 

which completes the proof. 
=-- 

=-- 


[[!redirects monoidal monads]]
